[Progress] Port disk layer to new generic structure.

src/DiskLayer/Definitions.v
@@ -1,12 +1,10 @@
-Require Import Primitives Simulation.
+Require Import Primitives Simulation Layer.
 Import ListNotations.
 
 Set Implicit Arguments.
 
 Definition hashmap := @mem hash hash_dec (hash * value).
 Definition encryptionmap := @mem value value_dec (key * value).
-  
-Section DiskLayer.  
   
   Inductive token :=
   | Key : key -> token
@@ -22,18 +20,16 @@ Section DiskLayer.
 
   Definition state := (((list key * encryptionmap)* hashmap) * disk (set value))%type.
   
-  Inductive prog : Type -> Type :=
-  | Read : addr -> prog value
-  | Write : addr -> value -> prog unit
-  | GetKey : list value -> prog key
-  | Hash : hash -> value -> prog hash
-  | Encrypt : key -> value -> prog value
-  | Decrypt : key -> value -> prog value
-  | Ret : forall T, T -> prog T
-  | Bind : forall T T', prog T -> (T -> prog T') -> prog T'.
+  Inductive op : Type -> Type :=
+  | Read : addr -> op value
+  | Write : addr -> value -> op unit
+  | GetKey : list value -> op key
+  | Hash : hash -> value -> op hash
+  | Encrypt : key -> value -> op value
+  | Decrypt : key -> value -> op value.
    
   Inductive exec :
-    forall T, oracle ->  state -> prog T -> @Result state T -> Prop :=
+    forall T, oracle ->  state -> op T -> @Result state T -> Prop :=
   | ExecRead : 
       forall m d a v,
         read d a = Some v ->
@@ -68,52 +64,67 @@ Section DiskLayer.
         consistent_with_upds em
              (map (encrypt k) vl) (map (fun v => (k, v)) vl) ->
         exec [Key k] (kl, em, hm, d) (GetKey vl) (Finished ((k::kl), em, hm, d) k)
-             
-  | ExecRet :
-      forall d T (v: T),
-        exec [Cont] d (Ret v) (Finished d v)
+ 
+  | ExecCrash :
+      forall T d (p: op T),
+        exec [Crash] d p (Crashed d).
 
-  | ExecBind :
-      forall T T' (p1: prog T) (p2: T -> prog T')
-        o1 d1 d1' o2 r ret,
-        exec o1 d1 p1 (Finished d1' r) ->
-        exec o2 d1' (p2 r) ret ->
-        exec (o1++o2) d1 (Bind p1 p2) ret
-
-  | ExecOpCrash :
-      forall T d (p: prog T),
-        (forall T' (p1: prog T') p2, p <> Bind p1 p2) ->
-        exec [Crash] d p (Crashed d)
-             
-  | ExecBindCrash :
-      forall T T' (p1: prog T) (p2: T -> prog T')
-        o1 d1 d1',
-        exec o1 d1 p1 (Crashed d1') ->
-        exec o1 d1 (Bind p1 p2) (Crashed d1').
-
-  Fixpoint oracle_ok {T} (p: prog T) o s :=
-    match p with
-    | Bind p1 p2 =>
-      exists o1 o2,
-      o = o1++o2 /\
-      oracle_ok p1 o1 s /\
-      (forall s' r,
-          exec o1 s p1 (Finished s' r) ->
-          oracle_ok (p2 r) o2 s') /\
-      (forall s',
-          exec o1 s p1 (Crashed s') ->
-          o2 = [])
-    | GetKey vl =>
+  Fixpoint oracle_ok T (p: op T) (o: oracle) (s: state) :=
+   match p with
+  | GetKey vl =>
       (exists k, ~In k (fst(fst(fst s))) /\
-            consistent_with_upds (snd(fst (fst s)))
+            @consistent_with_upds _ _ value_dec (snd(fst (fst s)))
                 (map (encrypt k) vl) (map (fun v => (k,v)) vl) /\
             o = [Key k]) \/ o = [Crash]
     | _ =>
       o = [Cont] \/ o = [Crash]
     end.
 
-  Definition layer1_lts := Build_LTS oracle state prog exec.
-End DiskLayer.
 
-Notation "x <- p1 ; p2" := (Bind p1 (fun x => p2))(right associativity, at level 60).
+  Theorem exec_deterministic_wrt_oracle :
+    forall o s T (p: op T) ret1 ret2,
+      exec o s p ret1 ->
+      exec o s p ret2 ->
+      ret1 = ret2.
+  Proof.
+    intros; destruct p; simpl in *; cleanup;
+    repeat
+      match goal with
+      | [H: exec _ _ _ _ |- _] =>
+        inversion H; clear H; cleanup
+      end; eauto.
+  Qed.
+
+  Theorem exec_then_oracle_ok:
+    forall T (p: op T) o s r,
+      exec o s p r ->
+      oracle_ok p o s.
+  Proof.
+    intros; destruct p; simpl in *; cleanup;
+    repeat
+      match goal with
+      | [H: exec _ _ _ _ |- _] =>
+        inversion H; clear H; cleanup
+      end; eauto.
+  Qed.
+  
+Module DiskOperation <: Operation.
+  Definition oracle := oracle.
+  Definition oracle_dec:= list_eq_dec token_dec.
+  Definition state := state.
+  Definition op := op.
+  Definition exec := exec.
+  Definition oracle_ok := oracle_ok.
+  Definition exec_deterministic_wrt_oracle :=
+    exec_deterministic_wrt_oracle.
+  Definition exec_then_oracle_ok :=
+    exec_then_oracle_ok.
+End DiskOperation.
+
+Module DiskHL := HoareLogic DiskOperation.
+Export DiskHL.
+
+Definition layer1_lts := Build_LTS DiskHL.L.oracle state DiskHL.L.prog DiskHL.L.exec.
+
+Notation "p >> s" := (p (snd s)) (right associativity, at level 60).
 Hint Constructors exec.
